LF_to_L section - main proof completed

LangEquivalence.v
@@ -1,49 +1,356 @@
+(* LL <-> LF (labeled <-> hybrid) *)
 Require Import Labeled.
 Require Import LabelFree.
 Require Import LibVar.
 Require Import LibLogic.
 Require Import LibList.
 Require Import LibListSorted.
+Require Import OkLib.
+Require Import LLOkLib.
 
 Open Scope labeled_is5_scope.
 Open Scope label_free_is5_scope.
+Open Scope is5_scope.
+Open Scope permut_scope.
 
-Section Contexts.
+Section LF_to_L.
 
-(* labeled from label-free *)
-Fixpoint annotate_worlds (w: var) (L: list (var * ty)) := 
-(* TODO: add explicit result type: Context_L (when possible) *)
-match L with 
+Fixpoint annotate_worlds (w: var) (L: list (var * ty)) : Context_L :=
+match L with
   | nil => nil
-  | (x, T) :: L' => (x, T, w) :: annotate_worlds w L'
+  | (x, T) :: L' => (w, (x, T)) :: annotate_worlds w L'
 end.
 
-Definition labeled_context (G: Background_LF) (Ctx:Context_LF) :=
-(* TODO: again, explicit result type when possible *)
-  let CtxLst := Ctx :: G in
-  let Omega := map fst CtxLst in
-  let Delta := flat_map (fun x => annotate_worlds (fst x) (snd x)) CtxLst in
+Definition labeled_context (G: Background_LF) (Ctx: Context_LF) :
+  (list var) * Context_L * var :=
+  let Omega := map fst_ (Ctx :: G) in
+  let Delta := flat_map (fun x => annotate_worlds (fst_ x) (snd_ x))
+    (Ctx :: G) in
   (Omega, Delta, fst Ctx).
 
+Fixpoint labeled_term (M0: te_LF) :=
+match M0 with
+| hyp_LF v =>
+  hyp_L v
+| lam_LF A M =>
+  lam_L A (labeled_term M)
+| appl_LF M N =>
+  appl_L (labeled_term M) (labeled_term N)
+| box_LF M =>
+  box_L (labeled_term M)
+| unbox_fetch_LF w M =>
+  unbox_L (fetch_L w (labeled_term M))
+| get_here_LF w M =>
+  get_L w (here_L (labeled_term M))
+| letdia_get_LF w M N =>
+  letd_L (get_L w (labeled_term M)) (labeled_term N)
+end.
+
+(* FIXME: move this :) *)
+Lemma ok_LF_not_Mem_fst:
+forall (G: Background_LF) U w,
+  ok_LF G U -> Mem w U ->
+  ~ Mem w (map fst_ G) .
+induction G; intros; simpl in *.
+rewrite Mem_nil_eq; auto.
+destruct a; rew_map; simpl; rewrite Mem_cons_eq; intro; destruct H1; subst.
+inversion H; subst; auto; inversion H; subst. apply IHG in H0;
+[ contradiction | ]; inversion H; subst; apply ok_LF_used_weakening in H7; auto.
+Qed.
+
+Lemma PPermut_map_fst:
+forall G G',
+  G ~=~ G' ->
+  map fst_ G *=* map fst_ G'.
+Admitted.
+
+Lemma PPermut_flat_map_annotate_worlds:
+forall G G',
+  G ~=~ G' ->
+  flat_map (fun x => annotate_worlds (fst_ x) (snd_ x)) G *=*
+  flat_map (fun x => annotate_worlds (fst_ x) (snd_ x)) G'.
+Admitted.
+
+(* until here *)
+
+Lemma ok_LF_impl_ok_Omega:
+forall G w Gamma Omega,
+  ok_LF ((w, Gamma)::G) nil ->
+  Omega *=* fst_ (fst_ (labeled_context G (w, Gamma))) ->
+  ok_Omega Omega.
+(*
+induction G; intros; inversion H; subst;
+[simpl in *; eauto | destruct a].
+unfold labeled_context; rew_map; simpl; repeat split.
+rewrite Mem_cons_eq; intro; destruct H0; subst; inversion H6; subst;
+[elim H4; apply Mem_here | ].
+simpl. apply ok_LF_not_Mem_fst with (w:=w) in H8;
+[contradiction | repeat rewrite Mem_cons_eq]; right; left; auto.
+inversion H6; subst;
+apply ok_LF_not_Mem_fst with (U:=v::w::nil); auto; apply Mem_here.
+assert (ok_Omega (map fst_ ((w, Gamma) :: G))).
+  apply IHG with (w:=w) (Gamma:=Gamma).
+  inversion H6; subst; constructor; auto.
+  apply ok_LF_used_weakening in H7; auto.
+  rew_map; simpl; symmetry; rew_map; simpl; auto.
+  rew_map in *; simpl in *; destruct H0; auto.
+*)
+Admitted.
+
+Lemma ok_LF_impl_ok_Gamma:
+forall G w Gamma Delta U,
+  ok_LF (flat_map snd_ ((w, Gamma)::G)) U ->
+  Delta *=* snd_ (fst_ (labeled_context G (w, Gamma))) ->
+  ok_Gamma Delta U.
+Admitted.
+
+Lemma ok_Bg_impl_ok_L:
+forall G w Gamma Omega Delta,
+  ok_Bg ((w, Gamma)::G) ->
+  Omega *=* fst_ (fst_ (labeled_context G (w, Gamma))) ->
+  Delta *=* snd_ (fst_ (labeled_context G (w, Gamma))) ->
+  ok_L Omega Delta.
+intros; destruct H; split;
+[eapply ok_LF_impl_ok_Omega |
+ eapply ok_LF_impl_ok_Gamma]; eauto.
+Qed.
+
+Lemma Mem_preserved_world_L:
+forall G w Gamma Omega Delta,
+  Omega *=* fst_ (fst_ (labeled_context G (w, Gamma))) ->
+  Delta *=* snd_ (fst_ (labeled_context G (w, Gamma))) ->
+  forall w0 Gamma0,
+    Mem (w0, Gamma0) ((w, Gamma)::G) ->
+    Mem w0 Omega.
+Admitted.
+
+Lemma Mem_preserved_term_L:
+forall G w Gamma Omega Delta,
+  Omega *=* fst_ (fst_ (labeled_context G (w, Gamma))) ->
+  Delta *=* snd_ (fst_ (labeled_context G (w, Gamma))) ->
+  forall w0 x0 a0 Gamma0,
+    Mem (w0, Gamma0) ((w, Gamma)::G) ->
+    Mem (x0, a0) Gamma0 ->
+    Mem  (w0, (x0, a0)) Delta.
+Admitted.
+
+Lemma subst_t_rewrite_L:
+forall M N x,
+  subst_t_L (labeled_term M) x (labeled_term N) =
+  labeled_term (subst_t M x N).
+Admitted.
+
+Lemma subst_w_rewrite_L:
+forall M w w',
+  subst_w_L (labeled_term M) w w' =
+  labeled_term (subst_w w w' M).
+Admitted.
+
+Lemma labeled_typing:
+forall G w Gamma M A Omega Delta w' M'
+  (HT: G |= (w, Gamma) |- M ::: A)
+  (H_Omega: Omega *=* fst_ (fst_ (labeled_context G (w, Gamma))))
+  (H_Delta: Delta *=* snd_ (fst_ (labeled_context G (w, Gamma))))
+  (H_w: w' = snd_ (labeled_context G (w, Gamma)))
+  (H_M: M' = labeled_term M),
+  Omega; Delta |- M' ::: A @ w.
+intros;
+unfold labeled_context in *; rew_flat_map in *; rew_map in *;
+simpl in *; subst;
+generalize dependent Omega;
+generalize dependent Delta;
+remember (w, Gamma) as Ctx;
+generalize dependent w;
+generalize dependent Gamma.
+induction HT;
+intros; inversion HeqCtx; subst; simpl in *.
+(* hyp *)
+apply t_hyp_L.
+  eapply ok_Bg_impl_ok_L; simpl; eauto.
+  eapply Mem_preserved_world_L with (w:=w0) (Gamma:=Gamma0);
+    simpl; eauto; eapply Mem_here.
+  eapply Mem_preserved_term_L with (w:=w0) (Gamma:=Gamma0);
+    simpl; eauto; eapply Mem_here.
+(* lam *)
+apply t_lam_L with (L:=L).
+  eapply ok_Bg_impl_ok_L; eauto.
+  intros. replace (hyp_L (fte x)) with (labeled_term (hyp_LF (fte x))).
+  unfold open_t_L; rewrite subst_t_rewrite_L. eapply H; eauto.
+  simpl; permut_simpl; auto.
+  simpl; auto.
+(* appl *)
+apply t_appl_L with (A:=A).
+  eapply ok_Bg_impl_ok_L; eauto.
+  eapply IHHT1; eauto.
+  eapply IHHT2; eauto.
+(* box *)
+apply t_box_L with (L:=L).
+  apply ok_Bg_impl_ok_L with (G:=G) (w:=w0) (Gamma:=Gamma0); auto;
+    assert ((w0, Gamma0) :: G ~=~ G & (w0, Gamma0)) as H1 by PPermut_simpl;
+    rewrite H1; auto.
+  eapply Mem_preserved_world_L with (w:=w0) (Gamma:=Gamma0);
+    simpl; eauto; eapply Mem_here.
+  intros; unfold open_w_L; rewrite subst_w_rewrite_L.
+  apply H with (Gamma:=nil); auto.
+  rewrite H_Delta; simpl; rew_app; rew_flat_map; simpl; permut_simpl.
+  rew_map; simpl; rewrite H_Omega; permut_simpl.
+(* unbox_fetch *)
+apply t_unbox_L.
+  eapply ok_Bg_impl_ok_L; eauto.
+  apply t_fetch_L.
+    eapply ok_Bg_impl_ok_L; eauto.
+    eapply IHHT; eauto.
+    apply Mem_permut with (l:=w0::map fst_ G);
+    [ symmetry | apply Mem_here ]; auto.
+apply t_unbox_L.
+  eapply ok_Bg_impl_ok_L; eauto.
+  simpl; rew_map; simpl; rewrite H_Omega; permut_simpl.
+  replace ((w::nil) ++ map fst_ G) with (map fst_ ((w, Gamma)::G))
+    by (rew_map; simpl; auto);
+  apply PPermut_map_fst; rewrite <- H; PPermut_simpl.
+  simpl; rewrite H_Delta; rew_flat_map; simpl; permut_simpl.
+  apply PPermut_flat_map_annotate_worlds in H; rew_map in *;
+    rewrite <- H; rew_flat_map; simpl; permut_simpl.
+  apply t_fetch_L.
+    eapply ok_Bg_impl_ok_L; eauto.
+    rewrite H_Omega; symmetry; simpl; rew_map; simpl; permut_simpl.
+    replace ((w::nil) ++ map fst_ G) with (map fst_ ((w, Gamma)::G))
+      by (rew_map; simpl; auto);
+    apply PPermut_map_fst; rewrite <- H; PPermut_simpl.
+    simpl; rewrite H_Delta; rew_flat_map; simpl; permut_simpl.
+    apply PPermut_flat_map_annotate_worlds in H; rew_map in *;
+      rewrite <- H; rew_flat_map; simpl; permut_simpl.
+    eapply IHHT; eauto.
+    simpl; rewrite H_Delta; rew_flat_map; simpl; permut_simpl.
+    apply PPermut_flat_map_annotate_worlds in H; rew_map in *;
+      rewrite <- H; rew_flat_map; simpl; permut_simpl.
+    rewrite H_Omega; rew_map; simpl; permut_simpl.
+    replace ((w::nil) ++ map fst_ G) with (map fst_ ((w, Gamma)::G))
+      by (rew_map; simpl; auto);
+    apply PPermut_map_fst; rewrite <- H; PPermut_simpl.
+    eapply Mem_preserved_world_L with (w:=w0) (Gamma:=Gamma0);
+    simpl; eauto; eapply Mem_here.
+(* get_here *)
+apply t_get_L.
+  eapply ok_Bg_impl_ok_L; eauto.
+  apply t_here_L.
+    eapply ok_Bg_impl_ok_L; eauto.
+    eapply IHHT; eauto.
+    apply Mem_permut with (l:=w0::map fst_ G);
+    [ symmetry | apply Mem_here ]; auto.
+apply t_get_L.
+  eapply ok_Bg_impl_ok_L; eauto.
+  simpl; rew_map; simpl; rewrite H_Omega; permut_simpl.
+  replace ((w::nil) ++ map fst_ G) with (map fst_ ((w, Gamma)::G))
+    by (rew_map; simpl; auto);
+  apply PPermut_map_fst; rewrite <- H; PPermut_simpl.
+  simpl; rewrite H_Delta; rew_flat_map; simpl; permut_simpl.
+  apply PPermut_flat_map_annotate_worlds in H; rew_map in *;
+    rewrite <- H; rew_flat_map; simpl; permut_simpl.
+  apply t_here_L.
+    eapply ok_Bg_impl_ok_L; eauto.
+    rewrite H_Omega; symmetry; simpl; rew_map; simpl; permut_simpl.
+    replace ((w::nil) ++ map fst_ G) with (map fst_ ((w, Gamma)::G))
+      by (rew_map; simpl; auto);
+    apply PPermut_map_fst; rewrite <- H; PPermut_simpl.
+    simpl; rewrite H_Delta; rew_flat_map; simpl; permut_simpl.
+    apply PPermut_flat_map_annotate_worlds in H; rew_map in *;
+      rewrite <- H; rew_flat_map; simpl; permut_simpl.
+    eapply IHHT; eauto.
+    simpl; rewrite H_Delta; rew_flat_map; simpl; permut_simpl.
+    apply PPermut_flat_map_annotate_worlds in H; rew_map in *;
+      rewrite <- H; rew_flat_map; simpl; permut_simpl.
+    rewrite H_Omega; rew_map; simpl; permut_simpl.
+    replace ((w::nil) ++ map fst_ G) with (map fst_ ((w, Gamma)::G))
+      by (rew_map; simpl; auto);
+    apply PPermut_map_fst; rewrite <- H; PPermut_simpl.
+    eapply Mem_preserved_world_L with (w:=w0) (Gamma:=Gamma0);
+    simpl; eauto; eapply Mem_here.
+(* letdia_get *)
+apply t_letd_L with (A:=A) (Lt:=L_t) (Lw:=L_w).
+  eapply ok_Bg_impl_ok_L; eauto.
+  apply t_get_L.
+    eapply ok_Bg_impl_ok_L; eauto.
+    eapply IHHT; eauto.
+    eapply Mem_preserved_world_L with (w:=w0) (Gamma:=Gamma0);
+    simpl; eauto; eapply Mem_here.
+  intros; unfold open_t in *; unfold open_w in *;
+  unfold open_t_L in *; unfold open_w_L in *.
+    rewrite subst_w_rewrite_L.
+    replace (hyp_L (fte t)) with (labeled_term (hyp_LF (fte t))).
+    rewrite subst_t_rewrite_L.
+    eapply H; eauto.
+    rewrite H_Delta; rew_map; simpl; permut_simpl.
+    rewrite H_Omega; rew_map; simpl; permut_simpl.
+    simpl; auto.
+apply t_letd_L with (A:=A) (Lt:=L_t) (Lw:=L_w).
+  eapply ok_Bg_impl_ok_L; eauto.
+  rewrite H_Omega; simpl; rew_map; simpl; permut_simpl;
+  replace ((w::nil) ++ map fst_ G) with (map fst_ ((w, Gamma)::G))
+    by (rew_map; simpl; auto);
+  apply PPermut_map_fst; rewrite <- H0; PPermut_simpl.
+  simpl; rewrite H_Delta; rew_flat_map; simpl; permut_simpl;
+  apply PPermut_flat_map_annotate_worlds in H0; rew_map in *;
+  rewrite <- H0; rew_flat_map; simpl; permut_simpl.
+  apply t_get_L.
+    eapply ok_Bg_impl_ok_L; eauto.
+    rewrite H_Omega; simpl; rew_map; simpl; permut_simpl;
+    replace ((w::nil) ++ map fst_ G) with (map fst_ ((w, Gamma)::G))
+      by (rew_map; simpl; auto);
+    apply PPermut_map_fst; rewrite <- H0; PPermut_simpl.
+    simpl; rewrite H_Delta; rew_flat_map; simpl; permut_simpl;
+    apply PPermut_flat_map_annotate_worlds in H0; rew_map in *;
+    rewrite <- H0; rew_flat_map; simpl; permut_simpl.
+    eapply IHHT; eauto.
+    simpl; rewrite H_Delta; rew_flat_map; simpl; permut_simpl;
+    apply PPermut_flat_map_annotate_worlds in H0; rew_map in *;
+    rewrite <- H0; rew_flat_map; simpl; permut_simpl.
+    rewrite H_Omega; simpl; rew_map; simpl; permut_simpl;
+    replace ((w::nil) ++ map fst_ G) with (map fst_ ((w, Gamma)::G))
+      by (rew_map; simpl; auto);
+    apply PPermut_map_fst; rewrite <- H0; PPermut_simpl.
+    eapply Mem_preserved_world_L with (w:=w0) (Gamma:=Gamma0);
+    simpl; eauto; eapply Mem_here.
+    intros; unfold open_t in *; unfold open_w in *;
+    unfold open_t_L in *; unfold open_w_L in *.
+    rewrite subst_w_rewrite_L.
+    replace (hyp_L (fte t)) with (labeled_term (hyp_LF (fte t))).
+    rewrite subst_t_rewrite_L.
+    eapply H; eauto.
+    simpl; rewrite H_Delta; rew_flat_map; simpl; permut_simpl;
+    apply PPermut_flat_map_annotate_worlds in H0; rew_map in *;
+    rewrite <- H0; rew_flat_map; simpl; permut_simpl.
+    rewrite H_Omega; simpl; rew_map; simpl; permut_simpl.
+    replace (map fst_ G & w) with (map fst_ (G & (w, Gamma)))
+      by (rew_map; simpl; auto);
+    apply PPermut_map_fst; rewrite <- H0; PPermut_simpl.
+    simpl; auto.
+Qed.
+
+End LF_to_L.
+
+Section L_to_LF.
+
 (* label-free from labeled *)
-Fixpoint filter_w (L: list (var * (var * ty))) (e: var) :=
+Fixpoint filter_w (L: Context_L) (e: var) :=
 match L with
 | nil => nil
-| v :: L' => 
-  If fst v = e then 
-    let (x, t) := snd v in
+| (w, (x, t)) :: L' =>
+  if (eq_var_dec e w) then
     (x, t) :: filter_w L' e
   else filter_w L' e
 end.
 
-Fixpoint label_free_context (Omega: list var) Gamma w : (Background_LF * Context_LF) :=
-match Omega with 
+Fixpoint label_free_context (Omega: list var) Gamma w :
+  Background_LF * Context_LF :=
+match Omega with
 | nil => (nil, (w, nil))
 | w0 :: Omega' =>
   let (G, Delta) := label_free_context Omega' Gamma w in
   let curr := filter_w Gamma w in
-  If w = w0 then 
-  (* we assume that Delta did not result in anything interesting -- we can do this
+  If w = w0 then
+  (* we assume that Delta did not result in anything interesting
+     -- we can do this if ok_L Omega Gamma
      because every world should be only once in Omega, so w should be there once
      as well - and this means that Delta = (w, nil) *)
     (G, (w, curr))
@@ -51,86 +358,41 @@ match Omega with
     ((w, curr) :: G, Delta)
 end.
 
-End Contexts.
-
-(*
-Section Terms.
-
-(* FIXME: this should be ctx_L in labeled/* code *)
-Definition ctx_L:=wo.
-
-Fixpoint labeled_world (w: ctx_LF) : (ctx_L) :=
-match w with
-| bctx n => bwo n
-| fctx w' => fwo w'
-end.
-
-Fixpoint label_free_world (w: ctx_L) : (ctx_LF) :=
-match w with
-| bwo n => bctx n
-| fwo w' => fctx w'
-end.
-(*
-
-Fixpoint labeled_var (v: var_LF) : (var_L) :=
-match v with
-| bvar_LF n => bvar_L n
-| fvar_LF v' => fvar_L v'
-end.
- 
-Fixpoint label_free_var (v: var_L) : (var_LF) :=
-match v with
-| bvar_L n => bvar_LF n
-| fvar_L v' => fvar_LF v'
-end.
-
-*)
-
-Fixpoint labeled_term (M0: te_LF) :=
+Fixpoint label_free_term (M0: te_L) (w: vwo) :=
 match M0 with
-| hyp_LF v => hyp_L 0 (* labeled_var v *)
-| lam_LF A M => lam_L (labeled_type A) (labeled_term M)
-| appl_LF M N => appl_L (labeled_term M) (labeled_term N)
-| box_LF M => box_L (labeled_term M)
-| unbox_fetch_LF w M => unbox_L (fetch_L (labeled_world w) (labeled_term M))
-| get_here_LF w M => get_L (labeled_world w) (here_L (labeled_term M))
-| letdia_get_LF w M N => letd_L (get_L (labeled_world w) (labeled_term M)) (labeled_term N)
+| hyp_L v =>
+  hyp_LF v
+| lam_L A M =>
+  lam_LF A (label_free_term M w)
+| appl_L M N =>
+  appl_LF (label_free_term M w)  (label_free_term N w)
+| box_L M =>
+  box_LF (label_free_term M w)
+| unbox_L M =>
+  unbox_fetch_LF w (label_free_term M w)
+| here_L M =>
+  get_here_LF w (label_free_term M w)
+| letd_L M N =>
+  letdia_get_LF w (label_free_term M w) (label_free_term N w)
+(* ? *)
+| get_L w0 M =>
+  letdia_get_LF w0 (label_free_term M w) (get_here_LF w0 (hyp_LF (bte 0)))
+(* note: do we need to ensure for fetch that w0 used down there is fresh? *)
+| fetch_L w0 M =>
+  box_LF (unbox_fetch_LF w0 (label_free_term M w0))
 end.
 
-Fixpoint label_free_term (M0: te_L) (w: ctx_LF) :=
-match M0 with
-| hyp_L v => hyp_LF (bvar 0) (* label_free_var v *)
-| lam_L A M => lam_LF (label_free_type A) (label_free_term M w)
-| appl_L M N => appl_LF (label_free_term M w)  (label_free_term N w)
-| box_L M => box_LF (label_free_term M w)
-| unbox_L M => unbox_fetch_LF w (label_free_term M w)
-| here_L M => get_here_LF w (label_free_term M w)
-| letd_L M N => letdia_get_LF w (label_free_term M w) (label_free_term N w)
-| get_L w0 M => letdia_get_LF (label_free_world w0) (label_free_term M w) 
-                             (get_here_LF (label_free_world w0) (hyp_LF 0))
-| fetch_L w0 M => box_LF (unbox_fetch_LF (label_free_world w0) (label_free_term M))
-end.
-
-End Terms.
-*)
-(*
-Lemma labeled_typing:
-forall G w Gamma M A Omega Delta M' A' w'
-  (HT: G |= (w, Gamma) |- M ::: A)
-  (H_Ctx: (Omega, Delta, w') = labeled_context G w Gamma) 
-  (H_M: M' = labeled_term M)
-  (H_A: A' = labeled_type A),
-  Omega; Delta |- M' ::: A' @ w'.
+Lemma ok_L_impl_ok_Bg:
+forall Omega Gamma w G Delta,
+  ok_L Omega Gamma ->
+  (G, (w, Delta)) = label_free_context Omega Gamma w ->
+  ok_Bg ((w, Delta)::G).
 Admitted.
 
 Lemma label_free_typing:
 forall Omega Gamma M A w G Delta M' A'
   (HT: Omega; Gamma |- M ::: A @ w)
-  (H_G: permut (label_free_context Omega Gamma) (G & (w, Delta)))
-  (H_M: M' = label_free_term M)
-  (H_A: A' = label_free_type A),
+  (H_G: label_free_context Omega Gamma w = (G, (w, Delta)))
+  (H_M: M' = label_free_term M (fwo w)),
   G |= (w, Delta) |- M' ::: A'.
 Admitted.
-*)
-Close Scope labeled_is5_scope.
-Close Scope label_free_is5_scope.
